templates/hindsight/hindsight_proof.v
@@ -11,78 +11,41 @@ Require Export hindsight flows.
 
 Module Type HINDSIGHT_SPEC (DS : DATA_STRUCTURE).
   Module DEFS := HINDSIGHT_DEFS DS.
-  Import DS.
+  Import DS DEFS.
 
-  Parameter dsOp_upd_spec: ∀ N γ_r γ_t γ_m γ_td1 γ_td2 γ_ght op (r: Node) 
-                          γ_sy t_id t0 Q,
-          DEFS.main_inv N γ_t γ_r γ_m γ_td1 γ_td2 γ_ght -∗
-          □ DEFS.update_helping_protocol N γ_t γ_r γ_td1 γ_td2 γ_ght -∗
-          DEFS.thread_vars γ_t γ_ght γ_sy t_id t0 -∗
-            {{{ DEFS.au N γ_r op Q }}} 
-                  dsOp (Op_to_val op) #r
+  Definition is_updating (pvs : list (val * val)) : Prop :=
+    Exists (λ x, ∃ v1, x.1 = (v1, #true)%V) pvs.
+  
+  Global Instance is_updating_dec : ∀ pvs, Decision (is_updating pvs).
+  Proof.
+    intros pvs. rewrite /is_updating. apply Exists_dec. intros [x1 x2].
+    rewrite /=. destruct x1.
+    - right; intros [v1 H']; try done.
+    - right; intros [v1 H']; try done.
+    - destruct (decide (x1_2 = #true)) as [-> | Hx1]. 
+      + left. by exists x1_1.
+      + right. intros [v1 H']. inversion H'. done.
+    - right; intros [v1 H']; try done.
+    - right; intros [v1 H']; try done.
+  Qed.
+
+  Parameter dsOp_spec: ∀ N γ_t γ_r γ_m γ_ght op r (p: proph_id) pvs 
+    γ_sy t_id t0 Q,
+          main_inv N γ_t γ_r γ_m γ_ght -∗
+          □ update_helping_protocol N γ_t γ_r γ_ght -∗
+            {{{ proph p pvs ∗ 
+                (⌜is_updating pvs⌝ ∗ au N γ_r op Q ∨
+                  ⌜¬ is_updating pvs⌝ ∗ thread_vars γ_t γ_ght γ_sy t_id t0) }}} 
+                  dsOp (Op_to_val op) #r #p
             {{{ (res: resT), RET #res; 
-                  if updater_thread op res then Q #res
-                  else DEFS.past_lin_witness γ_m op res t0 }}}.
-
-(*
-  Parameter dsOp_nupd_spec: ∀ N γ_r γ_t γ_m γ_td1 γ_td2 γ_ght op (r: Node) 
-                          γ_sy t_id t0,
-          DEFS.main_inv N γ_t γ_r γ_m γ_td γ_ght -∗
-          □ DEFS.update_helping_protocol N γ_t γ_r γ_td γ_ght -∗
-          DEFS.thread_vars γ_t γ_ght γ_sy t_id t0 -∗
-            {{{ True }}} 
-                  dsOp (Op_to_val op) #r
-            {{{ res, RET #res; DEFS.past_lin_witness γ_m op res t0 }}}.
-*)
+                  ⌜is_updating pvs⌝ ∗ Q #res
+                ∨ ⌜¬ is_updating pvs⌝ ∗ past_lin_witness γ_m op res t0 }}}.
 
 End HINDSIGHT_SPEC.
 
 Module CLIENT_SPEC (DS : DATA_STRUCTURE) (HS: HINDSIGHT_SPEC DS).
   Import DS HS.DEFS HS.
-  
-  (* Test zone *)
-  
-  Lemma test_and (P: iProp) : P -∗ P ∧ P.
-  Proof.
-    iIntros "HP". iSplit; try done.
-  Qed.
-  
-  Definition test_fn : val :=
-    λ: "l",
-      let: "p" := NewProph in
-      Resolve (!"l") "p" #1 ;;
-      #().
-      
-  Definition test_inv N l : iProp := inv (cntrN N) (l ↦ #2).
-  
-  Lemma test_spec N l :
-    test_inv N l -∗
-      <<< True >>> test_fn #l @ ⊤ <<< True, RET #() >>>.
-  Proof.
-    iIntros "#HInv" (Φ) "AU". wp_lam.
-    wp_apply wp_new_proph1; first done.
-    iIntros (p vp)"Hproph". wp_pures. wp_bind (Resolve _ _ _)%E.
-    iInv "HInv" as ">H'".
-    wp_apply (wp_resolve1 with "Hproph"); try done.  
-    wp_load. iModIntro.
-    iIntros "%". Search proph.
-    iModIntro. iSplitL "H'"; try iFrame.
-    wp_pures. iMod "AU" as "[_ [_ Hcl]]".
-    by iApply "Hcl".
-  Qed.
     
-    
-  (* Test zone end *)
-  
-
-  Definition dsOp' : val :=
-    λ: "OP" "r",     
-      let: "t_id" := NewProph in
-      let: "p" := NewProph in
-      let: "v" := dsOp "OP" "r" in
-      resolve_proph: "p" to: "v";;
-      "v".
-        
   (** Proofs *)
     
   Lemma history_sync γ_m (M: gmap nat (agreeR (ucmra_ofeO snapshotUR))) 
@@ -111,340 +74,276 @@ Module CLIENT_SPEC (DS : DATA_STRUCTURE) (HS: HINDSIGHT_SPEC DS).
   Qed.
   
 
-  Lemma dsOp'_spec N γ_s γ_t γ_m γ_td1 γ_td2 γ_ght op (r: Node) :
-          DEFS.main_inv N γ_t γ_s γ_m γ_td1 γ_td2 γ_ght -∗
-              <<< ∀∀ a, dsRep γ_s a >>> 
-                     dsOp' (Op_to_val op) #r @ ↑(cntrN N)
-              <<< ∃∃ a' res, dsRep γ_s a' ∗ ⌜seq_spec op a a' res⌝, 
+  Definition dsOp' : val :=
+    λ: "OP" "r",     
+      let: "t_id" := NewProph in
+      let: "p_upd" := NewProph in
+      let: "p" := NewProph in
+      let: "v" := dsOp "OP" "r" "p_upd" in
+      resolve_proph: "p" to: "v";;
+      "v".
+
+
+  Lemma dsOp'_spec N γ_t γ_r γ_m γ_ght op (r: loc) :
+          main_inv N γ_t γ_r γ_m γ_ght -∗
+              <<< ∀∀ a, dsRep γ_r a >>> 
+                     dsOp' (Op_to_val op) #r @ ↑(cntrN N) ∪ ↑(threadN N)
+              <<< ∃∃ a' res, dsRep γ_r a' ∗ ⌜seq_spec op a a' res⌝, 
                   RET #res >>>.
   Proof.
     iIntros "#HInv" (Φ) "AU". wp_lam. 
-    wp_pure credit:"Hc". wp_pure credit:"Hc1". wp_pures.
+    wp_pure credit:"Hc". wp_pure credit:"Hc'". wp_pures.
     wp_apply wp_new_proph1; try done.
     iIntros (tid vtid)"Htid". wp_pures.
+    wp_apply wp_new_proph; first done.
+    iIntros (pvs p1)"Hproph1". wp_pures.
     wp_apply (typed_proph_wp_new_proph1 resTTypedProph); first done.
-    iIntros (vp p)"Hproph". wp_pures.
+    iIntros (vp p2) "Hproph2". wp_pures.
     
-    destruct (decide (updater_thread op vp = true)) as [Upd_thr | Upd_thr].
-    - 
-    iApply fupd_wp. 
-    iInv "HInv" as (M0 T0 s0) "(>HCntr & >%Habs0 & >Hist & Help & Templ)".
-    iApply (lc_fupd_add_later with "Hc1"). iNext. 
-    iDestruct "Help" as (R1 R2 hγt)"(HR1 & HR2 & Hγt & 
-      Domm_hγt & Hstar1 & Hstar2)".
+    iAssert (update_helping_protocol N γ_t γ_r γ_ght)%I 
+        as "Upd_help". 
+    { iIntros (M T s)"%Dom_M Ds Prot".
+      iDestruct "Prot" as (R G)"(HG & Domm_G & Hstar)".
+      iAssert (dsRep γ_r (abs s) -∗
+        ([∗ set] t_id ∈ R, Reg N γ_t γ_r γ_ght t_id M) ={⊤ ∖ ↑cntrN N}=∗
+        (([∗ set] t_id ∈ R, Reg N γ_t γ_r γ_ght t_id (<[T+1:=s]> M))
+        ∗ dsRep γ_r (abs s)))%I as "H'".
+      { iIntros "Ds". 
+        iInduction R as [|tid' R' tid_notin_R IH] "HInd" using set_ind_L; 
+          auto using big_sepS_empty'.
+        rewrite (big_sepS_delete _ ({[tid']} ∪ R') tid'); last by set_solver.
+        rewrite (big_sepS_delete _ ({[tid']} ∪ R') tid'); last by set_solver.
+        assert (({[tid']} ∪ R') ∖ {[tid']} = R') as HR'. set_solver. rewrite HR'.
+        iIntros "(Htid & Hbigstar)". 
+        iMod ("HInd" with "[$Ds] Hbigstar") as "(H' & Ds)". iFrame "H'". 
+        iDestruct "Htid" as (γ_tk' γ_sy' Q' op' vp' t0' vtid')
+          "(Hproph & #Hthd & Hsy & #HthInv)".
+        iInv "HthInv" as (M'' T'')"Hstate".
+        iDestruct "Hstate" as "(>Hsy' & >%Dom_M'' & >%Ht0 & Hstate)".
+        iAssert (⌜M'' = M⌝)%I as %->.
+        { iPoseProof (own_valid_2 _ _ _ with "[$Hsy] [$Hsy']") as "%H'".
+          rewrite frac_agree_op_valid_L in H'. iPureIntro; symmetry; apply H'. }
+        assert (T'' = T) as ->.
+        { rewrite Dom_M in Dom_M''. apply gset_seq_eq in Dom_M''. done. }
+        iAssert (|={⊤ ∖ ↑cntrN N ∖ ↑threadN N}=> 
+            own γ_sy' (to_frac_agree (1 / 2) (<[T+1:=s]> M))
+          ∗ own γ_sy' (to_frac_agree (1 / 2) (<[T+1:=s]> M)))%I
+          with "[Hsy Hsy']" as ">(Hsy & Hsy')".
+        { iCombine "Hsy Hsy'" as "H'". 
+          iEval (rewrite <-frac_agree_op) in "H'".
+          iEval (rewrite Qp.half_half) in "H'".
+          iMod ((own_update (γ_sy') (to_frac_agree 1 M) 
+                        (to_frac_agree 1 (<[T+1 := s]> M))) with "[$H']") as "H'".
+          { apply cmra_update_exclusive. 
+            rewrite /valid /cmra_valid /= /prod_valid_instance.
+            split; simpl; try done. }
+          iEval (rewrite <-Qp.half_half) in "H'".
+          iEval (rewrite frac_agree_op) in "H'".  
+          iDestruct "H'" as "(Hsy & Hsy')". by iFrame. }
+        assert (dom (<[(T + 1)%nat:=s]> M) = gset_seq 0 (T + 1)) as Dom_M'.
+        { rewrite dom_insert_L Dom_M. apply set_eq_subseteq. split.
+          all: intros x; rewrite elem_of_union elem_of_singleton 
+            !elem_of_gset_seq; lia. }
+        assert (t0' ≤ T+1) as Ht0' by lia.
+        iDestruct "Hstate" as "[HPending | HDone]".
+        - iDestruct "HPending" as "(AU & >Hc & >%Past_W)".
+          destruct (decide (seq_spec op' (abs s) (abs s) vp'))
+            as [Hss | Hss].
+          + iApply (lc_fupd_add_later with "Hc"). iNext.
+            iMod "AU" as (c) "[DsR [_ Hcomm]]".
+            iAssert (⌜c = abs s⌝)%I as "%". 
+            { unfold dsRep, dsRepI.
+              iDestruct (own_valid_2 with "[$Ds] [$DsR]") as %H'.
+              rewrite frac_agree_op_valid_L in H'.
+              destruct H' as [_ H']; by iPureIntro. } subst c. 
+            iSpecialize ("Hcomm" $! (abs s) vp'). 
+            iMod ("Hcomm" with "[DsR]") as "HΦ".
+            { iFrame. by iPureIntro. }
+            iModIntro. iSplitL "Hsy HΦ". iNext. iExists (<[T+1:=s]> M), (T+1).
+            iFrame "∗%". iRight. iSplitL; last first. iPureIntro. exists (T+1). 
+            split. split; try done. by rewrite lookup_total_insert. by iLeft.
+            iModIntro. iFrame. iExists γ_tk', γ_sy', Q', op', vp', t0', vtid'.
+            iFrame "∗#%".
+          + iModIntro. iSplitL "AU Hc Hsy". iNext. iExists (<[T+1:=s]> M), (T+1).
+            iFrame "∗%". iLeft. iFrame. iPureIntro. 
+            { intros [t [Ht1 Ht2]]. destruct (decide (t = T+1)) as [-> | Ht].
+              rewrite lookup_total_insert in Ht2. done.
+              apply Past_W. exists t. split. lia. 
+              rewrite lookup_total_insert_ne in Ht2; try done. } 
+            iModIntro. iFrame. iExists γ_tk', γ_sy', Q', op', vp', t0', vtid'.
+            iFrame "∗#%".
+        - iDestruct "HDone" as "(HDone & >%PastW)".
+          iModIntro. iSplitL "HDone Hsy". iNext. iExists (<[T+1:=s]> M), (T+1).
+          iFrame "∗%". iRight. iSplitL; last first. iPureIntro.
+          { destruct PastW as [t [Ht1 Ht2]]. exists t. split. lia.
+            rewrite lookup_total_insert_ne. done. lia. } iFrame.
+          iModIntro. iFrame. iExists γ_tk', γ_sy', Q', op', vp', t0', vtid'.
+          iFrame "∗#%". }
+      iPoseProof ("H'" with "[$Ds] [$Hstar]") as ">(Hstar & Ds)".
+      iModIntro. iFrame. iExists R, G. iFrame. }
     
-    iAssert (¬ ⌜tid ∈ R1 ∪ R2⌝)%I as %H'.
-    { admit. }
-    assert (tid ∉ R1 ∪ R2) as tid_notin_R12 by done.
-    clear H'.
-    (*
-    iAssert (▷ (⌜tid ∉ R⌝ 
-            ∗ ([∗ set] t_id ∈ R, Reg N γ_t γ_s γ_ght t_id M0) 
-            ∗ proph1 tid vtid))%I with "[Hstar_reg Htid]" 
-            as "(>%tid_notin_R & Hstar_reg & Htid)".
-    { destruct (decide (tid ∈ R)); try done.
-      - iEval (rewrite (big_sepS_elem_of_acc _ (R) tid); 
-                            last by eauto) in "Hstar_reg".
-        iDestruct "Hstar_reg" as "(Hreg & Hstar_reg')".
-        iDestruct "Hreg" as (? ? ? ? ? ? ?)"(H' & _)".
-        iAssert (▷ False)%I with "[H' Htid]" as "HF".
-        iApply (proph1_exclusive tid with "[Htid]"); try done.
-        iNext. iExFalso; try done.
-      - iNext. iFrame. by iPureIntro. }
-    *)
-    
-    iMod (own_update γ_td1 (● R1) (● (R1 ∪ {[tid]})) with "[$HR1]") as "HR1".
-    { apply (auth_update_auth _ _ (R1 ∪ {[tid]})).
-      apply gset_local_update. set_solver. }
-    iMod (own_update γ_td1 (● (R1 ∪ {[tid]})) (● (R1 ∪ {[tid]}) ⋅ ◯ {[tid]}) 
-              with "[$HR1]") as "(HR1 & #FP_t)".
-    { apply (auth_update_dfrac_alloc _ (R1 ∪ {[tid]}) ({[tid]})).
-      apply gset_included. clear; set_solver. }
+    destruct (decide (is_updating pvs)) as [Hpvs | Hpvs].
+    - wp_apply (dsOp_spec with "[] [] [AU Hproph1]"); try done.
+      { iFrame "Hproph1". iLeft. iFrame "AU %". }
+      iIntros (res)"Hor". iDestruct "Hor" as "[Hor | Hor]"; last first.
+      { iDestruct "Hor" as "(% & _)". exfalso; try done. }
+      iDestruct "Hor" as "(_&HΦ)". wp_pures. 
+      wp_apply (typed_proph_wp_resolve1 resTTypedProph with "Hproph2"); try done.
+      { rewrite /typed_proph_from_val /=. by rewrite resT_proph_resolve. }
+      wp_pures. iModIntro. iIntros "_". wp_pures. done.
+    - iApply fupd_wp. 
+      iInv "HInv" as (M0 T0 s0) "(Ds & >%Habs0 & Hist & Help & Templ)".
+      iApply (lc_fupd_add_later with "Hc"). iNext. 
+      iDestruct "Help" as (R0 G0)"(HG & %Domm_G0 & Hstar)".
       
-    iMod (own_alloc (1)%Qp) as (γ_fr)"Hfr". { try done. }
-    iEval (rewrite <-Qp.half_half) in "Hfr".      
-    iEval (rewrite -(frac_op (1/2) (1/2))) in "Hfr". 
-    iDestruct "Hfr" as "(Hfr1 & Hfr2)". 
+      iAssert (¬ ⌜tid ∈ R0⌝)%I as %tid_notin_R0.
+      { iIntros "%H'". 
+        iEval (rewrite (big_sepS_elem_of_acc _ (R0) tid); 
+          last by eauto) in "Hstar".
+        iDestruct "Hstar" as "(H' & _)".
+        iDestruct "H'" as (? ? ? ? ? ? ?)"(H' & _)".
+        iApply (proph1_exclusive tid with "[Htid]"); try done. }
+            
+      iMod (own_alloc (to_frac_agree (1) (M0))) 
+              as (γ_sy)"Hfr_t". { try done. }        
+      iEval (rewrite <-Qp.half_half) in "Hfr_t".      
+      iEval (rewrite (frac_agree_op (1/2) (1/2) _)) in "Hfr_t". 
+      iDestruct "Hfr_t" as "(Hreg_sy1 & Hreg_sy2)".  
 
-    (*
-    iMod (own_alloc (to_frac_agree (1) (M0))) 
-            as (γ_sy)"Hfr_t". { try done. }        
-    iEval (rewrite <-Qp.half_half) in "Hfr_t".      
-    iEval (rewrite (frac_agree_op (1/2) (1/2) _)) in "Hfr_t". 
-    iDestruct "Hfr_t" as "(Hreg_sy1 & Hreg_sy2)".  
-    *)
-    
-    iDestruct "Domm_hγt" as %Domm_hγt.
-    set (<[ tid := to_agree (T0, γ_fr) ]> hγt) as hγt'.
-    iDestruct (own_update _ _ 
-      (● hγt' ⋅ ◯ {[ tid := to_agree (T0, γ_fr) ]})
-             with "Hγt") as ">Hγt".
-    { apply auth_update_alloc. 
-      rewrite /hγt'.
-      apply alloc_local_update; last done.
-      rewrite <-Domm_hγt in tid_notin_R12.
-      by rewrite not_elem_of_dom in tid_notin_R12. }
-    iDestruct "Hγt" as "(Hγt & #Hreg_gh)".
-    (*  
-    iMod (own_alloc (Excl ())) as (γ_tk) "Token"; first try done.
-    *)
-    iAssert (⌜map_max M0 = T0⌝)%I as %M_max. 
-    { by iDestruct "Hist" as (M0') "(_&_&%&_)". }
-    iDestruct "Hist" as (M0')"(H'&H'')". Check own_update.
-    iDestruct (own_update _ _ (● (MaxNat T0) ⋅ ◯ (MaxNat T0)) with "H'") 
-      as ">H1'".
-    { apply auth_update_alloc. apply max_nat_local_update. 
-      try done. }
-    iDestruct "H1'" as "(H' & #HfragT0)".
-    iAssert (hist γ_t γ_m M0 T0) with "[H' H'']" as "Hist".
-    { iExists M0'; iFrame. }
-    
-    iModIntro. iSplitR "Hproph Hfr1". iNext.
-    iExists M0, T0, s0. iFrame "∗%".
-      iExists (R1 ∪ {[tid]}), R2, hγt'. iFrame.
-      iSplitR. iPureIntro. subst hγt'.
-      apply leibniz_equiv. rewrite dom_insert.
-      rewrite Domm_hγt. clear; set_solver.
-      rewrite (big_sepS_delete _ (R1 ∪ {[tid]}) tid); last by set_solver.
-      iSplitR "Hstar1". unfold Reg_upd.
-      iExists γ_fr, Φ, op, vp, T0, vtid.
-      rewrite Upd_thr; iFrame "∗#". iSplitR. { by iPureIntro. }
-      iLeft. iFrame.
-      assert ((R1 ∪ {[tid]}) ∖ {[tid]} = R1) as H' 
-                  by (clear -tid_notin_R12; set_solver).
-      by rewrite H'.
+      iMod (own_alloc (Excl ())) as (γ_tk) "Token"; first try done.
+
+      set (<[ tid := to_agree (T0, γ_sy) ]> G0) as G0'.
+      iDestruct (own_update _ _ 
+        (● G0' ⋅ ◯ {[ tid := to_agree (T0, γ_sy) ]})
+               with "HG") as ">HG".
+      { apply auth_update_alloc. rewrite /G0'.
+        apply alloc_local_update; last done. apply not_elem_of_dom.
+        by rewrite Domm_G0 in tid_notin_R0. }
+      iDestruct "HG" as "(HG & #Hreg_gh)".
+
+      iAssert (⌜dom M0 = gset_seq 0 T0⌝)%I as %Dom_M0. 
+      { by iDestruct "Hist" as (M0') "(_&_&%&_)". }
+      iDestruct "Hist" as (M0')"(H'&H'')".
+      iDestruct (own_update _ _ (● (MaxNat T0) ⋅ ◯ (MaxNat T0)) with "H'") 
+        as ">H1'".
+      { apply auth_update_alloc. apply max_nat_local_update. try done. }
+      iDestruct "H1'" as "(H' & #HfragT0)".
+      iAssert (hist γ_t γ_m M0 T0) with "[H' H'']" as "Hist".
+      { iExists M0'; iFrame. }
       
-      iModIntro. wp_bind (dsOp _ _)%E.
-      
-      iAssert (update_helping_protocol N γ_t γ_s γ_td1 γ_td2 γ_ght)%I 
-        as "Upd_help". { admit. }
-      iAssert (thread_vars γ_t γ_ght γ_fr tid T0)%I as "#Thr_vars".
-      { iFrame "#". } 
-      wp_apply (dsOp_upd_spec with "[] [] [] []"); try done.
-      
-      iIntros (res)"HpastW". wp_pures.
-      wp_apply ((typed_proph_wp_resolve1 resTTypedProph 
-                  _ _ _ _ _ _ _ (res))
-        with "Hproph"); try done.
-      { unfold typed_proph_from_val; simpl. by rewrite resT_proph_resolve. }  
-      wp_pures. iModIntro. iIntros "%vp_eq_res". subst vp.
-      rewrite Upd_thr. wp_pures; try done.
-    
-    destruct (decide (updater_thread op vp = true)) as [Upd_thr | Upd_thr].
-    - iModIntro. iSplitR "AU Hproph". iNext.
-      iExists M0, T0, s0. iFrame "∗%".
-      iExists (R ∪ {[tid]}), hγt'. iFrame.
-      iSplitR. iPureIntro. subst hγt'.
-      apply leibniz_equiv. rewrite dom_insert.
-      rewrite Domm_hγt. clear; set_solver.
-      rewrite (big_sepS_delete _ (R ∪ {[tid]}) tid); last by set_solver.
-      iSplitR "Hstar_reg". unfold Reg.
-      iExists γ_tk, γ_sy, Φ, op, vp, T0, vtid.
-      rewrite Upd_thr; iFrame "∗#".
-      assert ((R ∪ {[tid]}) ∖ {[tid]} = R) as H' 
-                  by (clear -tid_notin_R; set_solver).
-      by rewrite H'.
-      
-      iModIntro. wp_bind (dsOp _ _)%E.
-      
-      iAssert (update_helping_protocol N γ_t γ_s γ_td γ_ght)%I as "Upd_help".
-      { admit. }
-      iAssert (thread_vars γ_t γ_ght γ_sy tid T0)%I as "#Thr_vars".
-      { iFrame "#". } 
-      wp_apply (dsOp_upd_spec with "[] [] [] [AU]"); try done.
-      
-      iIntros (res)"HpastW". wp_pures.
-      wp_apply ((typed_proph_wp_resolve1 resTTypedProph 
-                  _ _ _ _ _ _ _ (res))
-        with "Hproph"); try done.
-      { unfold typed_proph_from_val; simpl. by rewrite resT_proph_resolve. }  
-      wp_pures. iModIntro. iIntros "%vp_eq_res". subst vp.
-      rewrite Upd_thr. wp_pures; try done.
-    - rewrite not_true_iff_false in Upd_thr.
-      assert (∀ op c c' res, Decision (seq_spec op c c' res)) 
-        as seq_spec_dec. { apply seq_spec_dec. }
-      destruct (decide (seq_spec op (abs (M0 !!! T0)) (abs (M0 !!! T0)) vp))
-        as [Hss | Hss].
-      + 
-      iMod "AU" as (c) "[Cntr [_ Hcomm]]".
-      iAssert (⌜c = abs s0⌝)%I as "%". 
-      { unfold dsRep, dsRepI. Search own valid.
-        iDestruct (own_valid_2 with "[$Cntr] [$HCntr]") as %H'.
-        rewrite frac_agree_op_valid_L in H'.
-        destruct H' as [_ H']; by iPureIntro. } subst c. 
-      iSpecialize ("Hcomm" $! (abs s0) vp). 
-      iMod ("Hcomm" with "[Cntr]") as "HΦ".
-      { iFrame. apply leibniz_equiv in Habs0. 
-        rewrite Habs0 in Hss. by iPureIntro. }
-   
-      iAssert (past_lin M0 T0 op vp T0)%I as "Hpast".
-      { iPureIntro. exists T0. split; try done. }
+      iAssert (|={⊤ ∖ ↑cntrN N}=> dsRepI γ_r (abs s0) ∗ 
+        (inv (threadN N) (∃ M T, State γ_sy γ_tk (au N γ_r op Φ) Φ M T op vp T0)))%I
+        with "[Ds AU Hc' Hreg_sy1]" as "H'".
+      { destruct (decide (seq_spec op (abs (M0 !!! T0)) (abs (M0 !!! T0)) vp))
+          as [Hss | Hss].
+        - iMod "AU" as (c) "[DsR [_ Hcomm]]".
+          iAssert (⌜c = abs s0⌝)%I as "%". 
+          { unfold dsRep, dsRepI.
+            iDestruct (own_valid_2 with "[$Ds] [$DsR]") as %H'.
+            rewrite frac_agree_op_valid_L in H'.
+            destruct H' as [_ H']; by iPureIntro. } subst c. 
+          iSpecialize ("Hcomm" $! (abs s0) vp). 
+          iMod ("Hcomm" with "[DsR]") as "HΦ".
+          { iFrame. apply leibniz_equiv in Habs0. 
+            rewrite Habs0 in Hss. by iPureIntro. }
         
-      iMod (inv_alloc (threadN N) _
-            (∃ M T, State γ_sy γ_tk (au N γ_s op Φ) Φ M T op vp T0) 
-                                  with "[Hreg_sy1 Token]") as "#HthInv".
-      { iNext. iExists M0, T0. iFrame "Hreg_sy1".
-        iSplitR. by iPureIntro.
-        iRight. unfold Done. iFrame "Hpast".
-        by iRight. }
+          iAssert (past_lin M0 T0 op vp T0)%I as "Hpast".
+          { iPureIntro. exists T0. split; try done. }
+          
+          iMod (inv_alloc (threadN N) _ 
+            (∃ M T, State γ_sy γ_tk (au N γ_r op Φ) Φ M T op vp T0) 
+            with "[HΦ Hreg_sy1]") as "#HthInv".
+          { iNext. iExists M0, T0. iFrame "∗%". iSplitR. by iPureIntro.
+            iRight. iSplitL. by iLeft. iFrame "#". }
+          iModIntro; iFrame "∗#".
+        - iMod (inv_alloc (threadN N) _ 
+           (∃ M T, State γ_sy γ_tk (au N γ_r op Φ) Φ M T op vp T0) 
+            with "[AU Hc' Hreg_sy1]") as "#HthInv".
+          { iNext. iExists M0, T0. iFrame "∗%". iSplitR. by iPureIntro.
+            iLeft. iFrame "AU Hc'". iPureIntro. intros [t [Ht Hss']].
+            assert (t = T0) as -> by lia. done. }
+          iModIntro; iFrame "∗#". }
+      iDestruct "H'" as ">(Ds & #HthInv)".
+
+      iModIntro. iSplitR "Hproph1 Hproph2 Token". iNext.
+      iExists M0, T0, s0. iFrame "∗%".
+      iExists (R0 ∪ {[tid]}), G0'. iFrame.
+      iSplitR. iPureIntro. subst G0'. rewrite dom_insert_L.
+      clear -Domm_G0; set_solver.
+      rewrite (big_sepS_delete _ (R0 ∪ {[tid]}) tid); last by set_solver.
+      iSplitR "Hstar". 
+      iExists γ_tk, γ_sy, Φ, op, vp, T0, vtid. iFrame "∗#".
+      assert ((R0 ∪ {[tid]}) ∖ {[tid]} = R0) as H' 
+                by (clear -tid_notin_R0; set_solver).
+      by rewrite H'.
       
-      iAssert (update_helping_protocol N γ_t γ_s γ_td γ_ght)%I as "Upd_help".
-      { admit. }
-      iAssert (thread_vars γ_t γ_ght γ_sy tid T0)%I as "#Thr_vars".
+      iAssert (thread_vars γ_t γ_ght γ_sy tid T0)%I as "#Thd".
       { iFrame "#". }
-  
+    
+      iModIntro. wp_apply (dsOp_spec with "[] [] [Hproph1]"); try done.
+      { iFrame "Hproph1". iRight. iFrame "#%". }
       
-      iModIntro. iSplitR "Hproph HΦ". iNext.
-      iExists M0, T0, s0.  iFrame "∗%".
-      iExists (R ∪ {[tid]}), hγt'. iFrame.
-      iSplitR. iPureIntro. subst hγt'.
-      apply leibniz_equiv. rewrite dom_insert.
-      rewrite Domm_hγt. clear; set_solver.
-      rewrite (big_sepS_delete _ (R ∪ {[tid]}) tid); last by set_solver.
-      iSplitR "Hstar_reg". unfold Reg.
-      iExists γ_tk, γ_sy, Φ, op, vp, T0, vtid. rewrite Upd_thr. iFrame "∗#".
-      assert ((R ∪ {[tid]}) ∖ {[tid]} = R) as H' 
-                by (clear -tid_notin_R; set_solver).
-      by rewrite H'.  
-        
-      iModIntro.
-      wp_apply (dsOp_nupd_spec); try done.
-      iIntros (res)"Hres". wp_pures.
+      iIntros (res)"Hor". iDestruct "Hor" as "[Hor | Hor]".
+      { iDestruct "Hor" as "(%&_)"; exfalso; try done. }
+      
+      iDestruct "Hor" as "(_&#PastW)". wp_pures. 
       wp_apply ((typed_proph_wp_resolve1 resTTypedProph 
-                  _ _ _ _ _ _ _ (res))
-        with "Hproph"); try done.
-      { unfold typed_proph_from_val; simpl. by rewrite resT_proph_resolve. }
-      wp_pures. iModIntro. iIntros "->".
-      wp_pures. iModIntro. done.
-      + 
-      iMod (inv_alloc (threadN N) _
-              (∃ M T, State γ_sy γ_tk (au N γ_s op Φ) Φ M T op vp T0) 
-                                    with "[AU Hc Hreg_sy1]") as "#HthInv".
-      { iNext. iExists M0, T0. iFrame "Hreg_sy1".
-        iSplitR. { by iPureIntro. }
-        iLeft. unfold Pending. iFrame "AU Hc". 
-        unfold past_lin. iIntros "%Hpast". 
-        destruct Hpast as [t [H' Hss']].
-        assert (t = T0) as -> by lia. contradiction. }
-
-      iModIntro. iSplitR "Hproph Token". iNext.
-      iExists M0, T0, s0. iFrame "∗%".
-      iExists (R ∪ {[tid]}), hγt'. iFrame.
-      iSplitR. iPureIntro. subst hγt'.
-      apply leibniz_equiv. rewrite dom_insert.
-      rewrite Domm_hγt. clear; set_solver.
-      rewrite (big_sepS_delete _ (R ∪ {[tid]}) tid); last by set_solver.
-      iSplitR "Hstar_reg". unfold Reg.
-      iExists γ_tk, γ_sy, Φ, op, vp, T0, vtid. rewrite Upd_thr. iFrame "∗#".
-      assert ((R ∪ {[tid]}) ∖ {[tid]} = R) as H' 
-                  by (clear -tid_notin_R; set_solver).
-      by rewrite H'.
+                _ _ _ _ _ _ _ (res))
+        with "Hproph2"); try done.
+      { rewrite /typed_proph_from_val /= resT_proph_resolve. done. }
+    
+      wp_pures. iModIntro. iIntros "<-". wp_pure credit: "Hc1". 
+      wp_pure credit: "Hc2". 
+      iInv "HInv" as (M1 T1 s1) "(>Ds & >%Habs1 & >Hist & Help & Templ)".
+      iApply (lc_fupd_add_later with "Hc1"). iNext. 
+      iDestruct "Help" as (R1 G1)"(HG & %Domm_G1 & Hstar)".
       
-      iModIntro. wp_bind (dsOp _ _)%E.
-      
-      iAssert (update_helping_protocol N γ_t γ_s γ_td γ_ght)%I as "Upd_help".
-      { admit. }
-      iAssert (thread_vars γ_t γ_ght γ_sy tid T0)%I as "#Thr_vars".
-      { iFrame "#". } 
-      wp_apply (dsOp_nupd_spec); try done.
-      iIntros (res)"HpastW".
-      
-      wp_pures.
-      wp_apply ((typed_proph_wp_resolve1 resTTypedProph 
-                  _ _ _ _ _ _ _ (res))
-        with "Hproph"); try done.
-      { unfold typed_proph_from_val; simpl. by rewrite resT_proph_resolve. }  
-      wp_pures. iModIntro. iIntros "%vp_eq_res". subst vp.
-       
-      iApply fupd_wp.
-      iDestruct "HpastW" as "(%Upd_thr' & HpastW)".
-      
-      iInv "HthInv" as (M1_th T1_th)"(>Hth_sy & >% & Hth_or)".
-      iInv "HInv" as (M1 T1 s1) "(>HCntr & >%Habs1 & >Hist & Help & Templ)".
-      iDestruct "Help" as (R1 hγt1)"(>HR & >Hγt 
-                                  & >Domm_hγt & Hstar_reg)".
-      
-      iAssert (⌜tid ∈ R1⌝)%I as "%".
-      { iPoseProof (own_valid_2 _ _ _ with "[$HR] [$FP_t]") as "H'".
-        iDestruct "H'" as %H'.
-        apply auth_both_valid_discrete in H'.
-        destruct H' as [H' _].
-        apply gset_included in H'.
-        iPureIntro. set_solver. }
-      rename H into tid_in_R1.
-      
-      iAssert (⌜map_max M1 = T1⌝)%I as %M_max1. 
+      iAssert (⌜tid ∈ R1⌝)%I as "%tid_in_R1".
+      { iPoseProof (own_valid_2 _ _ _ with "[$HG] [$Hreg_gh]") as "%H'".
+        apply auth_both_valid_discrete in H'. destruct H' as [H' _].
+        apply dom_included in H'. rewrite dom_singleton_L -Domm_G1 in H'.
+        iPureIntro. clear -H'; set_solver. }
+    
+      iAssert (⌜dom M1 = gset_seq 0 T1⌝)%I as %Dom_M1. 
       { by iDestruct "Hist" as (M1') "(_&_&%&_)". }
 
-      iAssert (▷ (⌜M1_th = M1⌝ ∗ ⌜T1_th = T1⌝ 
-               ∗ ([∗ set] t_id ∈ R1, Reg N γ_t γ_s γ_ght t_id M1)
-               ∗ own (γ_sy) (to_frac_agree (1 / 2) M1_th) ))%I
-                with "[Hstar_reg Hth_sy]" as "(>% & >% & Hstar_reg & >Hth_sy)". 
-      { 
-        iEval (rewrite (big_sepS_elem_of_acc _ (R1) tid); 
-                                last by eauto) in "Hstar_reg".
-        iDestruct "Hstar_reg" as "(Hreg_t & Hstar_reg')".
-        iDestruct "Hreg_t" as (γ_tk' γ_sy' Q' op' vp' t0' vtid')
-                          "(Hreg_proph & >Hreg_gh' & >Hreg_sy & H')".
-        iDestruct "Hreg_gh'" as "(Hreg_gh' & #?)".
-        iCombine "Hreg_gh" "Hreg_gh'" as "H''".
-        iPoseProof (own_valid with "H''") as "Valid".
-        iDestruct "Valid" as %Valid.
-        rewrite auth_frag_valid in Valid.
-        apply singleton_valid in Valid.
-        apply to_agree_op_inv in Valid.
-        apply leibniz_equiv in Valid.
-        injection Valid; intros <- <-.
-
-
-        iAssert (⌜M1_th = M1 ∧ T1_th = T1⌝)%I as "(% & %)".
-        { iPoseProof (own_valid_2 _ _ _ with "[$Hth_sy] [$Hreg_sy]") 
-              as "V_M".
-          iDestruct "V_M" as %V_M.
-          apply frac_agree_op_valid in V_M. destruct V_M as [_ V_M].
-          iPureIntro. split; first by apply leibniz_equiv.
-          rewrite tid_in_R1. apply leibniz_equiv in V_M. by rewrite V_M. } 
-        subst M1_th T1_th.
-          
-        iSplitR. { by iPureIntro. } 
-        iSplitR. iNext; by iPureIntro.
-        iSplitR "Hth_sy". iApply "Hstar_reg'".
-        iNext. iExists γ_tk', γ_sy, Q', op', vp', T0, vtid'.
-        iFrame "∗#". by iNext. 
-      } subst M1_th T1_th.
-      
-      iEval (unfold past_lin_witness) in "HpastW".
-      (* iEval (rewrite Upd_thr) in "HpastW".*)
-
+      iInv "HthInv" as (M1_th T1_th)"(>Hth_sy & >%Dom_M1' & >%Ht0 & Hth_or)".
+      iApply (lc_fupd_add_later with "Hc2"). iNext. 
+      iAssert (⌜M1_th = M1⌝)%I as %->.
+      { rewrite (big_sepS_delete _ R1 tid); try done.
+        iDestruct "Hstar" as "(H' & _)". 
+        iDestruct "H'" as (? γ_sy' ?????)"(_&#H'&H''&_)".
+        iDestruct "Thd" as "(H1'&_)". iDestruct "H'" as "(H1''&_)".
+        iCombine "H1'" "H1''" as "H2'".
+        iPoseProof (own_valid with "H2'") as "%HV".
+        rewrite auth_frag_valid in HV. 
+        apply singleton_valid, to_agree_op_inv, leibniz_equiv in HV. 
+        inversion HV. subst γ_sy'.
+        iPoseProof (own_valid_2 _ _ _ with "[$H''] [$Hth_sy]") as "%H'".
+        rewrite frac_agree_op_valid_L in H'. iPureIntro; symmetry; apply H'. }
+      assert (T1_th = T1) as ->.
+      { rewrite Dom_M1' in Dom_M1. by apply gset_seq_eq. }
       iDestruct "Hth_or" as "[HPending | HDone]".
-      { iDestruct "HPending" as "(AU & Hc & >%HPending)".
-        iDestruct "HpastW" as (s) "(HpastW & %Hseq)".
-          iDestruct "HpastW" as (t)"(%T0_le_t & Ht)".
-          iDestruct "Hist" as (M1') "(H'&H''&H''')".
-          iDestruct (history_sync with "[$H''] [$Ht]") as "%M1'_t".
-          iDestruct "H'''" as %(H1' & _ & H1'' & H1''').
-          apply (H1'' t s) in M1'_t.
-          exfalso. apply HPending. exists t.
-          split.
-          + split; try done. apply elem_of_dom_2 in M1'_t.
-            by apply map_max_dom in M1'_t.
-          + rewrite !lookup_total_alt. rewrite M1'_t. by simpl. }
-      
-      iDestruct "HDone" as "(HDone & Hpast)".  
-      iDestruct "HDone" as "[HDone | >Hth_or]"; last first.
-      { iPoseProof (own_valid_2 _ _ _ with "[$Token] [$Hth_or]") as "%".
+      { iExFalso. iDestruct "HPending" as "(_&_&%HPending)".
+        iDestruct "PastW" as (s) "(#PastW & %Hseq)".
+        iDestruct "PastW" as (t)"(%T0_le_t & Ht)".
+        iDestruct "Hist" as (M1') "(H'&H''&H''')".
+        iPoseProof (history_sync with "[$H''] [$Ht]") as "%H'".
+        iDestruct "H'''" as "(_&%H''&_)". apply H'' in H'.
+        iPureIntro. apply HPending. exists t. split. split; try done.
+        apply elem_of_dom_2 in H'. rewrite Dom_M1 elem_of_gset_seq in H'. lia.
+        apply lookup_total_correct in H'. by rewrite H'. }
+    
+      iDestruct "HDone" as "(HDone & #PastW')".
+      iDestruct "HDone" as "[HΦ | Token']"; last first.
+      { iPoseProof (own_valid_2 _ _ _ with "[$Token] [$Token']") as "%".
         exfalso; try done. }
-        
-      iModIntro. iSplitR "HDone Hth_sy Token Hpast".
-      iExists M1, T1, s1; iFrame "∗%".
-      iNext. iExists R1, hγt1; iFrame.     
-
-      iModIntro. iSplitL "Token Hth_sy Hpast".
-      iNext. iExists M1, T1. iFrame "Hth_sy". 
-      iSplitR. by iPureIntro. iRight. iFrame "∗%".
-      by subst T1.
       
-      iModIntro. by wp_pures.
+      iModIntro. iSplitL "Hth_sy Token".
+      iNext. iExists M1, T1. iFrame "Hth_sy %". iRight. iFrame "#". by iRight.
+      iModIntro. iSplitR "HΦ". iNext. iExists M1, T1, s1; iFrame "∗%".
+      iExists R1, G1; iFrame "∗%".
+      done. Unshelve. all: try done. admit.
   Admitted.
   
 End CLIENT_SPEC.
